

HW 5

Kevin Lin

2/13/2026

1

We are given $X_i \in \{0, 1\}$ (0 means control, 1 means treatment) and Y_i be the outcome for observation i . Let $n_0 = \sum_{i=1}^n \mathbf{1}\{X_i = 0\}$ and $n_1 = \sum_{i=1}^n \mathbf{1}\{X_i = 1\}$ be the number of control and treatment observations, respectively. Let \bar{Y}_0 and \bar{Y}_1 be the sample means of the control and treatment groups, respectively, and $\hat{\sigma}_0^2$ and $\hat{\sigma}_1^2$ the sample variance, defined as

$$\hat{\sigma}_g^2 = \frac{1}{n_g - 1} \sum_{i: X_i = g} (Y_i - \bar{Y}_g)^2, \quad g \in \{0, 1\}$$

The pooled variance two sample t-statistic is given by:

$$t = \frac{\bar{Y}_1 - \bar{Y}_0}{s_p \sqrt{\frac{1}{n_0} + \frac{1}{n_1}}}$$

where the pooled standard deviation is:

$$s_p = \sqrt{\frac{(n_0 - 1)\hat{\sigma}_0^2 + (n_1 - 1)\hat{\sigma}_1^2}{n_0 + n_1 - 2}}$$

Lastly, we are given the linear regression model $Y = \beta_0 + \beta_1 X + \epsilon$.

- (a) We can show that the OLS slope estimate equals the difference between the sample mean of the two groups as follows:

OLS satisfies the normal equations:

$$\sum_{i=1}^n (Y_i - \hat{\beta}_0 - \hat{\beta}_1 X_i) = 0, \quad \sum_{i=1}^n X_i (Y_i - \hat{\beta}_0 - \hat{\beta}_1 X_i) = 0$$

We know the group means should be:

$$\bar{Y}_0 = \frac{1}{n_0} \sum_{i: X_i = 0} Y_i, \quad \bar{Y}_1 = \frac{1}{n_1} \sum_{i: X_i = 1} Y_i$$

Using the second normal equation and that X_i is binary ($X_i^2 = X_i$), we have:

$$\sum_{i=1}^n X_i Y_i - \hat{\beta}_0 \sum_{i=1}^n X_i - \hat{\beta}_1 \sum_{i=1}^n X_i = 0$$

Again, because X_i is binary, any summation terms with $X_i = 0$ will vanish, so we can simplify the above to:

$$\begin{aligned} \sum_{i:X_i=1} Y_i - \hat{\beta}_0 \sum_{i:X_i=1} 1 - \hat{\beta}_1 \sum_{i:X_i=1} 1 &= 0 \\ \sum_{i:X_i=1} Y_i - \hat{\beta}_0 n_1 - \hat{\beta}_1 n_1 &= 0 \\ \frac{1}{n_1} \sum_{i:X_i=1} Y_i &= \hat{\beta}_0 + \hat{\beta}_1 \\ \bar{Y}_1 &= \hat{\beta}_0 + \hat{\beta}_1 \end{aligned}$$

Now we go back to the first equation and simplify by splitting into their respective groups:

$$\begin{aligned} \sum_{i:X_i=0} (Y_i - \hat{\beta}_0) + \sum_{i:X_i=1} (Y_i - \hat{\beta}_0 - \hat{\beta}_1) &= 0 \\ \sum_{i:X_i=0} Y_i - n_0 \hat{\beta}_0 + \sum_{i:X_i=1} Y_i - n_1 \hat{\beta}_0 - n_1 \hat{\beta}_1 &= 0 \\ \sum_{i:X_i=0} Y_i + \sum_{i:X_i=1} Y_i &= (n_0 + n_1) \hat{\beta}_0 + n_1 \hat{\beta}_1 \end{aligned}$$

Substitute in the group means and the equation for \bar{Y}_1 :

$$\begin{aligned} n_0 \bar{Y}_0 + n_1 \bar{Y}_1 &= (n_0 + n_1) \hat{\beta}_0 + n_1 \hat{\beta}_1 \\ n_0 \bar{Y}_0 + n_1 (\hat{\beta}_0 + \hat{\beta}_1) &= (n_0 + n_1) \hat{\beta}_0 + n_1 \hat{\beta}_1 \\ n_0 \bar{Y}_0 &= n_0 \hat{\beta}_0 \\ \bar{Y}_0 &= \hat{\beta}_0 \end{aligned}$$

Finally, we can substitute $\hat{\beta}_0$ back into the equation for \bar{Y}_1 to get:

$$\begin{aligned} \bar{Y}_1 &= \bar{Y}_0 + \hat{\beta}_1 \\ \hat{\beta}_1 &= \bar{Y}_1 - \bar{Y}_0 \end{aligned}$$

which proves that the OLS slope estimate is the difference between the sample means of the two groups.

- (b) We can show that the OLS intercept estimate equals the sample mean of the control group in the same steps we took above with the first normal equation:

$$\begin{aligned} \sum_{i:X_i=0} (Y_i - \hat{\beta}_0) + \sum_{i:X_i=1} (Y_i - \hat{\beta}_0 - \hat{\beta}_1) &= 0 \\ \sum_{i:X_i=0} Y_i - n_0 \hat{\beta}_0 + \sum_{i:X_i=1} Y_i - n_1 \hat{\beta}_0 - n_1 \hat{\beta}_1 &= 0 \\ \sum_{i:X_i=0} Y_i + \sum_{i:X_i=1} Y_i &= (n_0 + n_1) \hat{\beta}_0 + n_1 \hat{\beta}_1 \end{aligned}$$

Substitute in the group means and the equation for \bar{Y}_1 :

$$\begin{aligned} n_0 \bar{Y}_0 + n_1 \bar{Y}_1 &= (n_0 + n_1) \hat{\beta}_0 + n_1 \hat{\beta}_1 \\ n_0 \bar{Y}_0 + n_1 (\hat{\beta}_0 + \hat{\beta}_1) &= (n_0 + n_1) \hat{\beta}_0 + n_1 \hat{\beta}_1 \\ n_0 \bar{Y}_0 &= n_0 \hat{\beta}_0 \\ \bar{Y}_0 &= \hat{\beta}_0 \end{aligned}$$

- (c) We can show that the homoscedastic OLS estimator of the error standard deviation equals the pooled standard deviation as follows: We know $\hat{Y}_i = \hat{\beta}_0 + \hat{\beta}_1 X_i$, so:

$$\hat{\sigma}^2 = \frac{1}{n-2} \sum_{i=1}^n (Y_i - \hat{\beta}_0 - \hat{\beta}_1 X_i)^2$$

We can split the above summation into the control and treatment groups:

$$\hat{\sigma}^2 = \frac{1}{n-2} \left(\sum_{i:X_i=0} (Y_i - \hat{\beta}_0)^2 + \sum_{i:X_i=1} (Y_i - \hat{\beta}_0 - \hat{\beta}_1)^2 \right)$$

Substitute in the equations for $\hat{\beta}_0$ and $\hat{\beta}_1$:

$$\hat{\sigma}^2 = \frac{1}{n-2} \left(\sum_{i:X_i=0} (Y_i - \bar{Y}_0)^2 + \sum_{i:X_i=1} (Y_i - \bar{Y}_1)^2 \right)$$

Recall that the corresponding within-group sample variances are:

$$\hat{\sigma}_0^2 = \frac{1}{n_0-1} \sum_{i:X_i=0} (Y_i - \bar{Y}_0)^2, \quad \hat{\sigma}_1^2 = \frac{1}{n_1-1} \sum_{i:X_i=1} (Y_i - \bar{Y}_1)^2$$

We can rearrange the above to get:

$$\sum_{i:X_i=0} (Y_i - \bar{Y}_0)^2 = (n_0 - 1) \hat{\sigma}_0^2, \quad \sum_{i:X_i=1} (Y_i - \bar{Y}_1)^2 = (n_1 - 1) \hat{\sigma}_1^2$$

Substitute the above into the equation for $\hat{\sigma}^2$:

$$\hat{\sigma}^2 = \frac{1}{n-2} ((n_0-1)\hat{\sigma}_0^2 + (n_1-1)\hat{\sigma}_1^2)$$

$$\hat{\sigma} = \sqrt{\frac{(n_0-1)\hat{\sigma}_0^2 + (n_1-1)\hat{\sigma}_1^2}{n-2}} = s_p$$

which proves that the homoscedastic OLS estimator of the error standard deviation equals the pooled standard deviation.

- (d) We can show that the OLS t-statistic for the slope estimate equals the two-sample t-statistic as follows:

We know our null hypothesis $H_0 : \beta_1 = 0$ and the OLS t-statistic is given by:

$$t_0 = \frac{\hat{\beta}_1}{\hat{se}(\hat{\beta}_1)}$$

We need to prove that:

$$\frac{\hat{\beta}_1}{\hat{se}(\hat{\beta}_1)} = \frac{\bar{Y}_1 - \bar{Y}_0}{s_p \sqrt{\frac{1}{n_0} + \frac{1}{n_1}}}$$

From the previous parts, we've already proved that $\hat{\beta}_1 = \bar{Y}_1 - \bar{Y}_0$ and $\hat{\sigma} = s_p$. We just need to show that $\hat{se}(\hat{\beta}_1) = s_p \sqrt{\frac{1}{n_0} + \frac{1}{n_1}}$. We know that the OLS standard error of the slope estimate is given by:

$$\hat{se}(\hat{\beta}_1) = \frac{\hat{\sigma}}{\sqrt{\sum_{i=1}^n (X_i - \bar{X})^2}}$$

Here, we know that $\bar{X} = \frac{n_1}{n_0+n_1}$ since X_i is binary. Then we have:

$$X_i = 0 : \quad X_i - \bar{X} = 0 - \frac{n_1}{n_0+n_1} = -\frac{n_1}{n_0+n_1}$$

$$X_i = 1 : \quad X_i - \bar{X} = 1 - \frac{n_1}{n_0+n_1} = \frac{n_0}{n_0+n_1}$$

Thus,

$$\begin{aligned}
\sum_{i=1}^n (X_i - \bar{X})^2 &= \sum_{i: X_i=0} \left(-\frac{n_1}{n_0 + n_1} \right)^2 + \sum_{i: X_i=1} \left(\frac{n_0}{n_0 + n_1} \right)^2 \\
&= n_0 \left(\frac{n_1}{n_0 + n_1} \right)^2 + n_1 \left(\frac{n_0}{n_0 + n_1} \right)^2 \\
&= \frac{n_0 n_1^2 + n_1 n_0^2}{(n_0 + n_1)^2} \\
&= \frac{n_0 n_1 (n_0 + n_1)}{(n_0 + n_1)^2} \\
&= \frac{n_0 n_1}{n_0 + n_1}
\end{aligned}$$

Plugging this back into our equation for $\hat{se}(\hat{\beta}_1)$, and applying our previous proof that $\hat{\sigma} = s_p$ we have:

$$\hat{se}(\hat{\beta}_1) = \frac{\hat{\sigma}}{\sqrt{\frac{n_0 n_1}{n_0 + n_1}}} = \hat{\sigma} \sqrt{\frac{n_0 + n_1}{n_0 n_1}} = s_p \sqrt{\frac{1}{n_0} + \frac{1}{n_1}}$$

- (e) In any finite sample, the OLS slope and intercept will always equal the difference in group means and the control group mean, respectively, regardless of the distribution of the error term ϵ . This comes algebraically from the linear model, the fact that X is binary, and the OLS normal equations. However, the OLS estimator of the error standard deviation will only equal the pooled standard deviation if the error term ϵ is homoscedastic. This is because the pooled variance formula assumes a common population variance across the two groups, which the homoscedastic OLS estimator of the error standard deviation also assumes. If the error term (grouped variances) differ, then the pooled t-test is invalid and the homoscedastic OLS SE is wrong, thus breaking the equality. Likewise, the t-statistic for the slope estimate will only equal the two-sample t-statistic if the error term is homoscedastic, since the OLS t-statistic relies on the pooled SE. It also requires that the correct degrees of freedom (in this case, $n - 2$) is used to calculate the OLS SE, which is the same as the degrees of freedom used to calculate the pooled SE (two degrees of freedom for β_0 , β_1 , and two degrees of freedom considering X_0 , X_1 where $(n_0 - 1) + (n_1 - 1) = n - 2$). If these assumptions are violated, then the OLS t-statistic will not equal the two-sample t-statistic.